Hash_alg for ecdsa

code/ecdsap256/Hacl.Interface.P256.fst
@@ -21,22 +21,26 @@ open Spec.P256
 open Spec.P256.Lemmas
 open Spec.P256.Definitions
 
+open Spec.ECDSA
 open Hacl.Impl.P256.Compression
 open Spec.Hash.Definitions
 
+open Hacl.Impl.ECDSA.P256SHA256.Signature.Agile
+
 
 let ecdsa_sign_p256_sha2 result mLen m privKey k = 
-  Hacl.Impl.ECDSA.P256SHA256.Signature.Agile.ecdsa_signature SHA2_256 result mLen m privKey k
+  ecdsa_signature (Hash SHA2_256) result mLen m privKey k
 
 let ecdsa_sign_p256_sha384 result mLen m privKey k = 
-  Hacl.Impl.ECDSA.P256SHA256.Signature.Agile.ecdsa_signature SHA2_384 result mLen m privKey k
+  ecdsa_signature (Hash SHA2_384) result mLen m privKey k
 
 let ecdsa_sign_p256_sha512 result mLen m privKey k = 
-  Hacl.Impl.ECDSA.P256SHA256.Signature.Agile.ecdsa_signature SHA2_512 result mLen m privKey k
+  ecdsa_signature (Hash SHA2_512) result mLen m privKey k
 
 let ecdsa_sign_p256_without_hash result m privKey k = 
-  Hacl.Impl.ECDSA.P256SHA256.Signature.Hashless.ecdsa_signature_without_hash result m privKey k
-
+  ecdsa_signature NoHash result 32ul m privKey k
+  
+(* 
 
 let ecdsa_verif_p256_sha2 mLen m pubKey r s = 
   Hacl.Impl.ECDSA.P256SHA256.Verification.Agile.ecdsa_verification SHA2_256 pubKey r s mLen m
@@ -78,3 +82,4 @@ let reduction_8_32 x result = Hacl.Impl.ECDSA.Reduction.reduction_8_32 x result
 let ecp256dh_i result scalar = Hacl.Impl.P256.DH.ecp256dh_i result scalar
 
 let ecp256dh_r result pubKey scalar = Hacl.Impl.P256.DH.ecp256dh_r result pubKey scalar
+ *)
