code/ecdsap256/Hacl.Interface.P256.ECDSA.fst
@@ -38,7 +38,7 @@ open Hacl.Impl.P256.Compression
 open Spec.Hash.Definitions
 open Hacl.Hash.Definitions
 
-
+(* 
 let ecdsa_sign_p256_sha2 result mLen m privKey k = 
   ecdsa_signature SHA2_256 result mLen m privKey k
 
@@ -49,8 +49,8 @@ let ecdsa_sign_p256_sha512 result mLen m privKey k =
   ecdsa_signature SHA2_512 result mLen m privKey k
 
 let ecdsa_sign_p256_without_hash result m privKey k = 
-  Hacl.Impl.ECDSA.P256SHA256.Signature.Hashless.ecdsa_signature_without_hash result m privKey k
-
+  ecdsa_signature NoHash result m privKey k
+(*  *)
 
 let ecdsa_verif_p256_sha2 mLen m pubKey r s = 
   Hacl.Impl.ECDSA.P256SHA256.Verification.Agile.ecdsa_verification SHA2_256 pubKey r s mLen m
@@ -86,3 +86,4 @@ let compressionCompressedForm b result =
  
 
 let reduction_8_32 x result = Hacl.Impl.ECDSA.Reduction.reduction_8_32 x result 
+ *)
